Proving CompileDFacade.v
--HG--
branch : facade

platform/facade/CompileDFacade.v
@@ -26,7 +26,15 @@ Fixpoint compile (s : Stmt) : Facade.Stmt :=
         (Facade.Call x (Var fun_ptr_varname) args)
   end.
 
-(*here*)
+Lemma compile_no_assign_to_args (spec : OperationalSpec) : is_disjoint (Facade.assigned (compile (Body spec))) (ArgVars spec) = true.
+  admit.
+Qed.
+
+Definition compile_op (spec : OperationalSpec) : Facade.OperationalSpec.
+  refine
+    (Facade.Build_OperationalSpec (ArgVars spec) (RetVar spec) (compile (Body spec)) (args_no_dup spec) (ret_not_in_args spec) _).
+  eapply compile_no_assign_to_args.
+Defined.
 
 Section ADTValue.
 
@@ -35,30 +43,167 @@ Section ADTValue.
   Notation State := (@State ADTValue).
   Notation Env := (@Env ADTValue).
   Notation Value := (@Value ADTValue).
+  Notation FuncSpec := (@FuncSpec ADTValue).
+  Notation RunsTo := (@RunsTo ADTValue).
+  Notation Safe := (@Safe ADTValue).
 
   Require Import Memory.
   Require Import GLabel.
 
   Notation FEnv := (@Facade.Env ADTValue).
+  Notation FFuncSpec := (@Facade.FuncSpec ADTValue).
+  Notation FRunsTo := (@Facade.RunsTo ADTValue).
+  Notation FSafe := (@Facade.Safe ADTValue).
 
-  Definition specs_fs_agree (env : Env) (env : Env) :=
-    let labels := fst env in
-    let fs := snd env in
-    forall p spec, 
-      fs p = Some spec <-> 
-      exists (lbl : glabel),
-        labels lbl = Some p /\
-        find lbl specs = Some spec.
+  Require Import GLabelMap.
+  Import GLabelMap.
 
-  Definition labels_in_scope (specs : Specs) (labels : glabel -> option W) :=
-    forall lbl, In lbl specs -> labels lbl <> None.
+  Arguments Facade.Operational {ADTValue} _.
 
-  Definition specs_stn_injective (specs : Specs) stn := forall lbl1 lbl2 (w : W), In lbl1 specs -> In lbl2 specs -> stn lbl1 = Some w -> stn lbl2 = Some w -> lbl1 = lbl2.
+  Definition compile_spec (spec : FuncSpec) : FFuncSpec :=
+    match spec with
+      | Axiomatic s => Facade.Axiomatic s
+      | Operational s => Facade.Operational (compile_op s)
+    end.
 
-  Definition specs_env_agree (specs : Specs) (env : Env) :=
-    labels_in_scope specs (fst env) /\
-    specs_stn_injective specs (fst env) /\
-    specs_fs_agree specs env.
+  Definition fenv_impls_env (fenv : FEnv) (env : Env) :=
+    forall lbl spec,
+      find lbl env = Some spec ->
+      exists w,
+        Label2Word fenv lbl = Some w /\
+        Word2Spec fenv w = Some (compile_spec spec).
+    
+  Require Import GeneralTactics4.
+  Require Import GeneralTactics3.
 
+  Require Import StringMap.
+  Import StringMap.
+  Require Import StringMapFacts.
+  Import FMapNotations.
+  Local Open Scope fmap_scope.
 
+  Require Import ListFacts4.
 
+  Require Import Setoid.
+  Add Morphism FRunsTo 
+      with signature (@eq FEnv) ==> (@eq Facade.Stmt) ==> (@Equal Value) ==> (@Equal Value) ==> iff as FRunsTo_m.
+    admit.
+  Qed.
+
+  Require Import StringSet.
+
+  Definition only_diff_in elt (m1 m2 : t elt) s := forall k v1 v2, find k m1 = Some v1 -> find k m2 = Some v2 -> m1 <> m2 -> StringSet.In k s.
+
+  Coercion string2elt (x : string) : StringSet.elt := x.
+  Coercion StringSet.singleton : StringSet.elt >-> StringSet.t.
+
+  Definition equiv (a b : State) := only_diff_in a b fun_ptr_varname.
+
+  Lemma equiv_refl st : equiv st st.
+    admit.
+  Qed.
+
+  Require Import Option.
+
+  Theorem compile_runsto : 
+    forall t t_env st st', 
+      FRunsTo t_env t st st' -> 
+      forall s, 
+        t = compile s -> 
+        is_syntax_ok s = true -> 
+        forall s_env, 
+          fenv_impls_env t_env s_env -> 
+          Safe s_env s st -> 
+          exists s_st',
+            RunsTo s_env s st s_st' /\
+            equiv s_st' st'. 
+  Proof.
+    induction 1; simpl; destruct s; unfold_all; simpl in *; try solve [intros; try discriminate]; intros Hcomp Hsyn s_env Henv Hsf.
+    {
+      (* skip *)
+      exists st.
+      split.
+      - eapply RunsToSkip; eauto.
+      - eapply equiv_refl; eauto.
+    }
+    {
+      Lemma is_syntax_ok_seq_elim a b : is_syntax_ok (Seq a b) = true -> is_syntax_ok a = true /\ is_syntax_ok b = true.
+        admit.
+      Qed.
+
+      (* seq *)
+      inject Hcomp.
+      inversion Hsf; subst.
+      destruct H4 as [Hsf1 Hsf2].
+      rename H into Hrt1.
+      rename H0 into Hrt2.
+      eapply is_syntax_ok_seq_elim in Hsyn.
+      destruct Hsyn as [Hsyn1 Hsyn2].
+      edestruct IHRunsTo1 as [s_st' [Hsst' Heq']]; eauto.
+      edestruct IHRunsTo2 as [s_st'' [Hsst'' Heq'']]; eauto.
+      (*here*)
+      eapply Hsf2; eauto.
+      eapply
+      eapply RunsToSeq; eauto.
+    }
+    {
+      (* call *)
+      inject Hcomp.
+      rename H into Hrtlbl.
+      rename H0 into Hrtcall.
+      inversion Hrtlbl; subst.
+      rename H1 into Hlw.
+      rename H2 into Hnadt.
+      rename H5 into Hst'.
+      rewrite Hst' in Hrtcall.
+      inversion Hrtcall; unfold_all; subst.
+      {
+        (* axiomatic *)
+        rename H3 into Hfw.
+        rename H4 into Hspec.
+        rename H5 into Hmm.
+        rename H6 into Hnadt2.
+        rename H7 into Hpre.
+        rename H8 into Hlen.
+        rename H11 into Hpost.
+        rename H12 into Hst''.
+        inversion Hsf; subst.
+        {
+          eapply RunsToCallAx.
+        
+
+    }
+    {
+      (* if-true *)
+      inject Hcomp.
+      inversion Hsf; subst; rename H5 into He; rename H6 into Hsfbr.
+      - eapply RunsToIfTrue; eauto.
+      - exfalso; eapply is_true_is_false; eauto.
+    }
+    {
+      (* if-false *)
+      inject Hcomp.
+      inversion Hsf; subst; rename H5 into He; rename H6 into Hsfbr.
+      - exfalso; eapply is_true_is_false; eauto.
+      - eapply RunsToIfFalse; eauto.
+    }
+    {
+      (* while-true *)
+      inject Hcomp.
+      inversion Hsf; unfold_all; subst.
+      - eapply RunsToWhileTrue; eauto.
+      - exfalso; eapply is_true_is_false; eauto.
+    }
+    {
+      (* while-false *)
+      inject Hcomp.
+      inversion Hsf; unfold_all; subst.
+      - exfalso; eapply is_true_is_false; eauto.
+      - eapply RunsToWhileFalse; eauto.
+    }
+    {
+      (* assign *)
+      inject Hcomp.
+      eapply RunsToAssign; eauto.
+    }
+  Qed.
